-

snake.v
@@ -4,95 +4,7 @@ Require Import Utf8.
 Require Import Classes.RelationClasses.
 Require Import Setoid.
 
-Reserved Notation "x '∈' S" (at level 60).
-Reserved Notation "x '≡' y" (at level 70).
-
-(* Abelian Groups.
-
-   Notes:
-
-   -sets in groups are predicates (naive theory of sets); a value of type
-    gr_set is not necessarily in the group set. To be in the group set, it
-    must satisfy the predicate gr_mem, which is later syntaxified by the
-    usual symbol ∈.
-
-   -group sets are setoids: there is a specific equality (gr_eq) which is
-    compatible with membership (gr_mem_compat), addition (gr_add_compat),
-    and inverse (gr_inv_compat). This allows to define quotient groups,
-    for example in cokernets, by changing this equality.
-*)
-
-Record AbGroup :=
-  { (* data *)
-    gr_set : Type;
-    gr_mem : gr_set → Prop where "x ∈ G" := (gr_mem x);
-    gr_eq : gr_set → gr_set → Prop where "x ≡ y" := (gr_eq x y);
-    gr_zero : gr_set where "0" := (gr_zero);
-    gr_add : gr_set → gr_set → gr_set where "x + y" := (gr_add x y);
-    gr_inv : gr_set → gr_set where "- x" := (gr_inv x);
-    (* properties *)
-    gr_zero_mem : 0 ∈ G;
-    gr_add_mem : ∀ x y, x ∈ G → y ∈ G → x + y ∈ G;
-    gr_add_0_l : ∀ x, 0 + x ≡ x;
-    gr_add_assoc : ∀ x y z, (x + y) + z ≡ x + (y + z);
-    gr_inv_mem : ∀ x, x ∈ G → - x ∈ G;
-    gr_add_inv_r : ∀ x, x + (- x) ≡ 0;
-    gr_add_comm : ∀ x y, x + y ≡ y + x;
-    gr_equiv : Equivalence gr_eq;
-    gr_mem_compat : ∀ x y, x ≡ y → x ∈ G → y ∈ G;
-    gr_add_compat : ∀ x y x' y', x ≡ y → x' ≡ y' → x + x' ≡ y + y';
-    gr_inv_compat : ∀ x y, x ≡ y → - x ≡ - y }.
-
-(* coq stuff: implicit and renamed arguments *)
-
-Arguments gr_eq [_].
-Arguments gr_zero [_].
-Arguments gr_add [_].
-Arguments gr_inv [_].
-Arguments gr_zero_mem G : rename.
-Arguments gr_add_mem G : rename.
-Arguments gr_add_0_l G : rename.
-Arguments gr_add_assoc G : rename.
-Arguments gr_inv_mem G : rename.
-Arguments gr_add_inv_r G : rename.
-Arguments gr_add_comm G : rename.
-Arguments gr_equiv G : rename.
-Arguments gr_mem_compat G : rename.
-Arguments gr_add_compat G : rename.
-Arguments gr_inv_compat G : rename.
-
-(* syntaxes for expressions for groups elements and sets *)
-
-Delimit Scope group_scope with G.
-
-Notation "0" := (gr_zero) : group_scope.
-Notation "a = b" := (gr_eq a b) : group_scope.
-Notation "a ≠ b" := (¬ gr_eq a b) : group_scope.
-Notation "a + b" := (gr_add a b) : group_scope.
-Notation "a - b" := (gr_add a (gr_inv b)) : group_scope.
-Notation "- a" := (gr_inv a) : group_scope.
-
-Notation "x '∈' S" := (gr_mem S x) (at level 60).
-Notation "x '∉' S" := (¬ gr_mem S x) (at level 60).
-
-Open Scope group_scope.
-
-(* Homomorphism between groups *)
-
-Record HomGr (A B : AbGroup) :=
-  { H_app : gr_set A → gr_set B;
-    H_mem_compat : ∀ x, x ∈ A → H_app x ∈ B;
-    H_app_compat : ∀ x y,
-      x ∈ A → y ∈ A → (x = y)%G → (H_app x = H_app y)%G;
-    H_additive : ∀ x y,
-      x ∈ A → y ∈ A → (H_app (x + y) = H_app x + H_app y)%G }.
-
-(* coq stuff: implicit and renamed arguments *)
-
-Arguments H_app [A] [B].
-Arguments H_mem_compat _ _ f : rename.
-Arguments H_app_compat _ _ f : rename.
-Arguments H_additive _ _ f : rename.
+Require Import AbGroup.
 
 (* Equality (gr_eq) in groups is an equivalence relation *)
 
@@ -1439,7 +1351,7 @@ split.
  now apply H_inv, Hg₁.
 Qed.
 
-(* The final lemma
+(* The snake lemma
                 f      g       cz
             A------>B------>C------>0
             |       |       |
@@ -1448,6 +1360,12 @@ Qed.
             v       v       v
      0----->A'----->B'----->C'
        za'      f'      g'
+
+  If 1/ the diagram is commutative,
+     2/ (f, g, cz) and (za', f', g') are exact sequences,
+  Then
+     there exists a morphism d from Ker c to Coker a, such that
+     Ker a→Ker b→Ker c→Coker a→Coker b→Coker c is an exact sequence.
 *)
 
 Lemma snake :
