five.v
@@ -1,0 +1,39 @@
+(* Five lemma *)
+
+Require Import Utf8.
+Require Import AbGroup.
+
+(* The five lemma
+         f      g       h        j
+     A------>B------>C------>D------>E
+     |       |       |       |       |
+    a|      b|      c|      d|      e|
+     |       |       |       |       |
+     v       v       v       v       v
+     A'----->B'----->C'----->D'----->E'
+        f'      g'      h'      j'
+
+  If 1/ the diagram is commutative,
+     2/ (f, g, h, j) and (f', g', h', j') are exact
+     3/ b and d are isomorphisms
+     4/ a is an epimorphism
+     5/ e is a monomorphism
+  Then
+     c is an isomorphism.
+*)
+
+Lemma five :
+  ∀ (A B C D E A' B' C' D' E' : AbGroup)
+     (f : HomGr A B) (g : HomGr B C) (h : HomGr C D) (j : HomGr D E)
+     (f' : HomGr A' B') (g' : HomGr B' C')
+     (h' : HomGr C' D') (j' : HomGr D' E'),
+  diagram_commutes f a b f'
+  → diagram_commutes g b c g'
+  → diagram_commutes h c d h'
+  → diagram_commutes j d e j'
+  → exact_sequence (Seq f (Seq g (Seq h (Seq j SeqEnd))))
+  → exact_sequence (Seq f' (Seq g' (Seq h' (Seq j' SeqEnd))))
+  → is_iso b ∧ is_iso d ∧ is_epi a ∧ is_mono e
+  → is_iso c.
+Proof.
+...
